027-flip_case.dfy
@@ -1,13 +1,13 @@
-predicate lower(c: char)
+function lower(c: char) : bool
     {
         'a' <= c <= 'z'
     }
 
-predicate upper(c: char)
+function upper(c: char) : bool
     {
         'A' <= c <= 'Z'
     }
-predicate alpha(c: char)
+function alpha(c: char) : bool
     {
         lower(c) || upper(c)
     }
@@ -20,14 +20,14 @@ function flip_char(c: char) : (C: char)
         if upper(c) then c + 'a' - 'A' else c
     }
 
-    function flip_case(s: string) : (S: string)
-        // post-conditions-start
-        ensures |S| == |s|
-        ensures forall i :: 0 <= i < |s| ==> (lower(s[i]) <==> upper(S[i]))
-        ensures forall i :: 0 <= i < |s| ==> (upper(s[i]) <==> lower(S[i]))
-        // post-conditions-end
-        {
+method flip_case(s: string) returns (S: string)
+    // post-conditions-start
+    ensures |S| == |s|
+    ensures forall i :: 0 <= i < |s| ==> (lower(s[i]) <==> upper(S[i]))
+    ensures forall i :: 0 <= i < |s| ==> (upper(s[i]) <==> lower(S[i]))
+    // post-conditions-end
+    {
         // impl-start
-            seq(|s|, i requires 0 <= i < |s| => flip_char(s[i]))
+        return seq(|s|, i requires 0 <= i < |s| => flip_char(s[i]));
         // impl-end
-        }
+    }
