080-is_happy.dfy
@@ -4,7 +4,7 @@ function ThreeDistinct(s: string, i: int): bool
     (s[i - 1] != s[i]) && (s[i] != s[i + 1]) && (s[i - 1] != s[i + 1])
 }
 
-predicate Happy(s: string)
+function Happy(s: string) : bool
 {
     |s| >= 3 &&
     forall i :: 0 < i < |s| - 1 ==> ThreeDistinct(s, i)
