098-count_upper.dfy
@@ -23,6 +23,6 @@ method count_upper(s: string) returns (cnt: int)
   // impl-end
 }
 
-predicate is_upper_vowel(c: char) {
+function is_upper_vowel(c: char) : bool {
   c == 'A' || c == 'E' || c == 'U' || c == 'I' || c == 'O'
 }
