104-unique_digits.dfy
@@ -1,4 +1,4 @@
-predicate HasNoEvenDigit(n: int)
+function HasNoEvenDigit(n: int) : bool
   decreases n
 {
   n >= 0 && ((n < 10 && n % 2 == 1) || (n % 2 == 1 && HasNoEvenDigit(n / 10)))
