109-move_one_ball.dfy
@@ -1,4 +1,4 @@
-predicate is_sorted(a: seq<int>) {
+function is_sorted(a: seq<int>) : bool {
   forall i, j :: 0 <= i < j < |a| ==> a[i] <= a[j]
 }
 
